Vcg.v
@@ -109,7 +109,7 @@ Fixpoint tc (c : com) (m : Sigma.sigma)
     match c with
     | CSkip => forall m', m = m' -> suite m'
     | CAss x a => forall m', (m' = set m x (aeval m a)) -> suite m'
-    | CAssert b => forall m', b m -> m = m' -> suite m'
+(*    | CAssert b => forall m', b m -> m = m' -> suite m'*)
     | CSeq p1 p2 => tc p1 m ps (fun m' => tc p2 m' ps suite)
     | CIf b p1 p2 =>
                 (*tc p1 m ps (fun m1' => 
@@ -236,7 +236,7 @@ Fixpoint tc' (c : com) (m : Sigma.sigma)
     match c with
     | CSkip => tc c m ps suite
     | CAss x a => tc c m ps suite
-    | CAssert b => b m /\ tc c m ps suite
+(*    | CAssert b => b m /\ tc c m ps suite*)
     | CSeq p1 p2 => tc' p1 m ps (fun m' => tc' p2 m' ps suite)
     | CIf b p1 p2 => 
          (bassn b m -> tc' p1 m ps (fun _ => True)) /\
@@ -250,7 +250,7 @@ Fixpoint tc' (c : com) (m : Sigma.sigma)
       tc c m m' ps suite*)
     end.
 
-Definition truc3 : com := CSeq (CAssert (fun m => m EAX = 2))
+(*Definition truc3 : com := CSeq (CAssert (fun m => m EAX = 2))
                           (CAssert (fun m => m EAX = 2)).
 
 Lemma test6 : forall m, (m EAX = 2) -> tc' truc3 m  empty_phi (fun _ => True).
@@ -276,4 +276,4 @@ split.
   * split.
     - auto.
     - split. all: try auto.
-Qed.
+Qed.*)
