Rela.v
@@ -1,0 +1,187 @@
+From Rela Require Import Vcg.
+From Rela Require Import Com.
+From Rela Require Import Bexp.
+From Rela Require Import Sigma.
+From Rela Require Import Hoare_Triple.
+
+Require Import Program.
+Require Import Eqdep_dec.
+From Coq Require Import Lists.List.
+Import ListNotations.
+From Coq Require Import Lia.
+
+(** Definition of assertion **)
+
+Definition r_assertion : Type := list sigma  -> Prop.
+
+Inductive rceval : list com -> list sigma -> Psi.psi -> list sigma -> Prop :=
+  | E_Empty : forall ps,
+      rceval [] [] ps []
+ | E_Seq : forall c qc s q s' q' ps,
+      ceval c s ps s' ->
+      rceval qc q ps q' ->
+      rceval (c::qc) (s::q) ps (s'::q').
+
+Definition relational_prop (P Q: r_assertion) (c : list com) (ps : Psi.psi) : Prop := 
+ forall s s',  length s = length c -> length s' = length c ->
+               P s -> rceval c s ps s' -> Q s'.
+
+Section play_ground.
+
+Lemma list_length_one:
+forall (A: Type) (h:A) (q : list A), length (h :: q) = 1 -> q = [].
+Proof.
+intros.
+simpl in H.
+apply eq_add_S in H.
+apply length_zero_iff_nil in H.
+assumption.
+Qed.
+
+Lemma rela_hoare :
+forall P Q c ps,
+hoare_triple (fun s => P [s]) (fun s => Q [s]) c ps ->
+relational_prop P Q [c] ps.
+Proof.
+unfold hoare_triple.
+unfold relational_prop.
+intros.
+inversion H3;subst.
+apply list_length_one in H0.
+apply list_length_one in H1.
+subst.
+eapply H.
+apply H2.
+assumption.
+Qed.
+
+End play_ground.
+
+Program Fixpoint rtc (cl : list com) (ml: list Sigma.sigma)
+            (ps: Phi.phi) (suite : list Sigma .sigma -> Prop) 
+            (hy:length cl = length ml): Prop :=
+ match cl ,ml with
+ | [],[] => suite []
+ | c :: qc, m :: qm => 
+   tc c m ps (fun m' => rtc qc qm ps (fun l => suite (m'::l))  _)
+ | _, _ => !
+end.
+
+Next Obligation.
+destruct cl.
+- simpl in hy.
+  symmetry in hy.
+  apply length_zero_iff_nil in hy.
+  subst ml.
+  contradiction H0.
+  split.
+  reflexivity.
+  reflexivity.
+- destruct ml as [|m qm].
+  discriminate hy.
+  eapply H.
+  split.
+  reflexivity.
+  reflexivity.
+Qed.
+
+Next Obligation.
+split.
+intros.
+intros contra.
+destruct contra as (contra & _).
+discriminate contra.
+intros contra.
+destruct contra as ( _ & contra).
+discriminate contra.
+Defined.
+
+Next Obligation.
+split.
+intros.
+intros contra.
+destruct contra as (_ & contra ).
+discriminate contra.
+intros contra.
+destruct contra as (contra & _).
+discriminate contra.
+Defined.
+
+Lemma mk_rtc_def :
+forall P h q pi s sl (hy:length (h::q) = length (s::sl)),
+exists (hyr:length q = length sl),
+rtc (h :: q) (s::sl) pi P hy  =
+tc h s pi (fun m' => rtc q sl pi (fun l => P (m'::l)) hyr).
+Proof.
+intros.
+eexists.
+program_simpl.
+Qed.
+
+Lemma hoare_rela :
+forall (P Q: r_assertion) h q ps pi sl (hy:length q = length sl), 
+(forall s2 s3 : sigma,
+P (s2 :: sl) -> ceval h s2 ps s3 -> 
+rtc q sl pi (fun sl : list sigma => Q (s3 :: sl)) hy) =
+hoare_triple (fun s => P (s:: sl) ) 
+             (fun s' => rtc q sl pi (fun sl : list sigma => Q (s' :: sl)) hy)
+              h ps.
+Proof.
+intros.
+unfold hoare_triple.
+reflexivity.
+Qed.
+
+Lemma correct :
+forall ps pi,
+forall p (P Q: r_assertion),
+(forall ml (hy:length p = length ml), 
+P ml -> rtc p ml pi Q hy) -> 
+relational_prop P Q p ps.
+Proof.
+intros ps pi p.
+unfold relational_prop.
+induction p.
+*  intros.
+   specialize (H []).
+   simpl in H.
+   apply length_zero_iff_nil in H0.
+   apply length_zero_iff_nil in H1.
+   subst.
+   apply H.
+   reflexivity.
+   assumption.
+*  intros.
+   destruct s.
+   + discriminate H0.
+   + destruct s'.
+   - discriminate H1.
+   - inversion H3;subst.
+    specialize (IHp (fun sl => P (s :: sl)) (fun sl => Q (s1 :: sl))).
+    simpl in IHp.
+    generalize H12.
+    generalize H2.
+    inversion H0.
+    inversion H1.
+    generalize H6.
+    generalize H5.
+    eapply IHp.
+    intros.
+    generalize H9.
+    generalize H4.
+    generalize s s1.
+    rewrite hoare_rela.
+    eapply (correct _ _ pi).
+    intros.
+    assert (hy2: length (a ::p) = length (m::ml)).
+    {intros. simpl. rewrite hy. reflexivity. }
+    destruct (mk_rtc_def Q a p pi m ml hy2) as (hyr & HYP).
+    specialize (H (m::ml) hy2).
+    rewrite HYP in H.
+    replace hy with hyr.
+    apply H.
+    assumption.
+    apply eq_proofs_unicity.
+    intros.
+    lia.
+Qed.
